promise_free/examples/MPAll.v
@@ -4,31 +4,13 @@ Require Import SystemHeader SystemI SystemA SystemIA SystemTactics.
 Require Import MPI MPA MPIA.
 Require Import Language.
 
-Module MPAll.
-  Import inv_instances.
+Section MPAux.
+  Context `{!crisG Γ Σ α β τ Hsub Hinv, !concGS, !histGS, !atomicG, !sysGS, !one_shotG}.
 
   Definition lang := Language.mk (λ _ : (), tt) (const False) (λ _ : ProgramEvent.t, λ _ _, True).
   Definition syn : Threads.syntax := IdentMap.singleton 1%positive (existT lang tt).
   Definition init : Configuration.t := Configuration.init syn [].
 
-  Local Instance Γ : HRA := ##[invΓ; concΓ; histΓ; atomicΓ; sysΓ; one_shotΓ].
-  Local Instance Σ : GRA := ##[Γ; invΣ].
-
-  Definition irΓ : Γ := **[ir_invΓ; ir_concΓ; PFMemA.ir_histΓ; *[None]; ir_sysΓ; *[None]].
-  Definition irΣ : Σ := **[irΓ; ir_invΣ].
-
-  Lemma irΣ_valid : ✓ (irΣ ⋅ ir_own_admin).
-  Proof.
-    solve_ir_valid.
-    - apply ir_tidRA_valid.
-    - apply ir_yieldRA_valid.
-    - apply PFMemA.ir_viewR_valid.
-    - apply PFMemA.ir_histR_valid.
-    - apply PFMemA.ir_hist_freeableUR_valid.
-    - apply ir_sysRA_valid.
-  Qed.
-
-  (* source module *)
   Local Definition sp_user_s : specmap := MPA.sp.
   Local Definition smod_src : SMod.t := (MPA.Mod) ☆ (SystemA.Mod sp_user_s ⊤) ☆ (PFMemA.smod).
   Local Definition mod_top : Mod.t := SMod.to_mod ∅ (SMod.cancel smod_src).
@@ -50,36 +32,6 @@ Module MPAll.
   Qed.
 
   Local Definition MainInSp : (MPA.sp) ⊆ sp_user_s. Proof. refl. Qed.
-
-  Lemma mod_top_wf : Mod.wf mod_top.
-  Proof.
-    rewrite /mod_top ?SMod.cancel_add ?SMod.to_mod_add. eapply Mod.add_wf.
-    { econs; eauto.
-      rewrite /MPA.Mod /= /MPA.fnsems /Mod.fnsems /= !fmap_insert !fmap_empty; mod_tac ss.
-    }
-    { econs; eauto.
-      { eapply Mod.add_wf.
-        { econs; eauto.
-          { rewrite /SystemA.Mod /= /SystemA.fnsems /Mod.fnsems /=
-              !fmap_insert !fmap_empty; mod_tac ss. }
-          { rewrite /= /SystemA.scopes; multiset_solver. }
-        }
-        { econs; eauto.
-          { rewrite /PFMemA.smod /= /PFMemA.fnsems /Mod.fnsems /=
-              !fmap_insert !fmap_empty; mod_tac ss. }
-          { rewrite /= /PFMemA.scopes; multiset_solver. }
-        }
-        { set_solver. }
-        { set_solver. }
-      }
-      { rewrite /=; i; rewrite multiplicity_disj_union /SystemA.scopes /PFMemA.scopes.
-        multiset_solver.
-      }
-    }
-    { rewrite !Mod.dom_fnsems_add; set_solver. }
-    { set_solver. }
-  Qed.
-
   Local Definition init_cond : iProp Σ := PFMemA.init_cond ∗ SystemA.init_cond [].
 
   (* Apply cancellation to linked spec module *)
@@ -94,7 +46,6 @@ Module MPAll.
     { apply SMod.cancellable_add; last apply SMod.cancellable_add; r;
         rewrite /= /MPA.fnsems /SystemA.fnsems /PFMemA.fnsems; mod_tac ss.
     }
-    { apply mod_top_wf. }
     { assert (Ht : SMod.conc_sp_from smod_src !! speckey_entry =
        fsp_some (MPA.main_spec)); last (rewrite Ht; clear Ht).
       { rewrite lookup_insert_ne // lookup_kmap_Some; exists None; split; ss. }
@@ -110,13 +61,11 @@ Module MPAll.
   Proof.
     eapply ctxr_refines.
     rewrite /mod_src /mod_tgt /smod_src !SMod.to_mod_add.
-
     (* abstraction of Mem *)
     etrans; cycle 1.
     { do 2 ctxr_drop.
       eapply PFMemIA.ctxr.
     }
-
     (* abstraction of Sch *)
     etrans; cycle 1.
     { ctxr_drop.
@@ -125,14 +74,12 @@ Module MPAll.
       - apply SchInSp.
       - rewrite dom_insert elem_of_union; left; apply elem_of_singleton; ss.
     }
-
     (* abstraction of MP *)
     etrans; cycle 1.
     { ctxr_norm. eapply MPIA.ctxr.
       - apply SchInSp.
       - apply MainInSp.
     }
-    
     eapply ctxr_cond_strengthen.
     { iIntros "[? [? ?]]". iFrame. }
   (*SLOW*)Qed.
@@ -176,33 +123,36 @@ Module MPAll.
     { rewrite !Mod.dom_fnsems_add; set_solver. }
     { set_solver. }
   Qed.
-  Hint Unfold sys_inG subG_sysG : GRA_index.
-  Lemma init_cond_valid :
-    ∃ rs, ✓ rs ∧ (Own rs ⊢ |==> init_cond ∗ TID 0 ∗ YIELD 0 ∗ winv (⊤, ⊤) ∗
-        tview_sys_gen 1 1 0 (TView.init []) ∗ TIDAUTH 0 ∗ YIELDAUTH 1).
-  Proof.
-    exists (irΣ ⋅ ir_own_admin). split.
-    - apply irΣ_valid.
-    - simplify_res.
-      { rewrite make_own_admin.
-        iDestruct "H22" as "[H22 Htid]". iFrame.
-        iPoseProof (PFMemA.make_init_cond with "[$]") as "[$ ?]".
-        rewrite big_sepM_singleton; iFrame.
-        iPoseProof (make_sys_init with "[$] [$]") as "[$ [$ [$ $]]]". done.
-      }
-    all: solve_res.
-  Qed.
+End MPAux.
+
+Module MPAll.
+  Import inv_instances.
+
+  Local Instance Γ : HRA := ##[invΓ; concΓ; histΓ; atomicΓ; sysΓ; one_shotΓ].
+  Local Instance Σ : GRA := ##[Γ; invΣ].
 
   Theorem behavioral_refinement :
-    ∃ src_res tgt_res, refines_lmod
-      (Mod.to_lmod mod_top src_res)
-      (Mod.to_lmod mod_tgt tgt_res).
+    ∃ β τ (Hinv : invGS Γ Σ α) (_ : crisG Γ Σ α β τ _ Hinv) (_ : concGS) (_ : histGS) (_ : sysGS)
+      src_res tgt_res,
+        refines_lmod
+          (Mod.to_lmod mod_top src_res)
+          (Mod.to_lmod mod_tgt tgt_res).
   Proof.
-    move: (top_tgt)=>H; rewrite /refines in H; des; ss.
-    hexploit H; eauto using tgt_wf. clear H; intros [WF H].
-    assert (IV:= init_cond_valid). des.
-    destruct (H rs); des; et.
-    rewrite IV0.
-    rewrite {1}winv_split_empty. iIntros ">[$ [$ [$ [[$ $] $]]]]". done.
+    apply own_admin_soundness.
+    iMod winv_alloc as "[% [% [% [% ?]]]]"; iExists _, _, _, _.
+    iMod conc_alloc as "[% ?]"; iExists _.
+    iMod hist_alloc as "[% [? TV]]"; iExists _.
+    iMod (sys_alloc with "TV") as "[% [? ?]]"; iExists _.
+    pose proof (top_tgt) as Href.
+    iStopProof. eapply entails_pointwise; iIntros (res Hres) "R".
+    iPoseProof (Own_valid with "R") as "%".
+    rewrite /refines in Href; hexploit Href; eauto using tgt_wf.
+    clear Href; intros [? Href].
+    iPureIntro; hexploit (Href res); eauto.
+    { rewrite Hres; iIntros "[W [[$ [$ [$ $]]] [[$ $] [$ $]]]]".
+      rewrite {1}winv_split_empty comm //.
+    }
+    intros [rt ?].
+    exists res, rt; by des.
   (*SLOW*)Qed.
 End MPAll.
